Source/DafnyStandardLibraries/src/Std/Parsers/Core/ParsersBuilders.dfy
@@ -16,10 +16,11 @@
 abstract module Std.Parsers.Builders {
   import P: Core
   export
+    provides Input
     provides P
     provides O
-    provides Return
-    provides Throw
+    provides SucceedWith
+    provides FailWith
     provides Rec
     provides B.e_I
     provides B.I_e
@@ -28,126 +29,267 @@ abstract module Std.Parsers.Builders {
     provides B.If
     provides B.?
     provides B.??
-    provides B.Commit
+    provides B.Then
+    provides B.ThenWithRemaining
+    provides B.Bind
     provides B.Rep
     provides B.RepSep
     provides B.RepMerge
     provides B.RepSepMerge
-    provides B.ZeroOrMore
-    provides B.OneOrMore
+    provides B.Rep1
     provides B.Debug
     provides End
+    provides Nothing
     provides IntToString
-    reveals CharTest
+    provides CharTest
+    reveals C
+    reveals ParseResult
     reveals B
     reveals Rec, RecMap
     reveals RecMapDef, FailureLevel, RecMapSel
 
+  type Input = P.Input
+  type C = P.C
+
+  /** `FailureLevel` is an alias for `P.FailureLevel`. Recoverable or Fatal */
   type FailureLevel = P.FailureLevel
+  /** A mapping from string to a parser returning `A` */
   type RecMapSel<A> = string -> B<A>
+  /** `ParseResult` is an alias for `P.ParseResult`. */
+  type ParseResult<+T> = P.ParseResult<T>
 
-  function Return<T>(t: T): B<T> {
-    B(P.Succeed(t))
-  }
-  function Throw<T>(message: string, level: FailureLevel := P.Recoverable): B<T> {
-    B(P.Fail(message,  level))
+
+  /** `SucceedWith(a)` returns success on any input,
+      `.value` contains the provided value.*/
+  function SucceedWith<T>(t: T): B<T> {
+    B(P.SucceedWith(t))
   }
 
-  // Wrap the constructor in a class where the size is constant so that users
-  // don'result need to provide it.
+  /** `FailWith(message)` returns a failure on any input, and does not consume input. */
+  function FailWith<T>(message: string, level: FailureLevel := P.Recoverable): B<T> {
+    B(P.FailWith(message,  level))
+  }
+
+  /** Parses nothing, always returns a success with nothing consumed. Can be useful in alternatives. */
+  const Nothing: B<()> := B(P.Epsilon())
+
+  /** Adapter to wrap any underlying parser so that they can be chained together. */
   datatype B<R> = B(apply: P.Parser<R>)
   {
+    /** `a.?()` evaluates `a` on the input, and then  
+        - If `a` succeeds, then wraps its result with `Some(...)`  
+        - If `a` fails, and the failure is not fatal and did not consume input, succeeds with `None`.  
+          If the error is fatal or did consume input, fails with the same failure.*/
     function ?(): B<P.Option<R>> {
       B(P.Maybe(apply))
     }
+
+    /** `a.??()` evaluates `a` on the input, and then  
+        - If `a` succeeds, returns the result unchanged.  
+        - If `a` fails, and the failure is not fatal, propagate the same failure but without consuming input.  
+         `a.??()` is useful when there are other alternatives to parse and a parsed partially and we are ok with trying something else. */
     function ??(): B<R> {
       B(P.?(apply))
     }
+
+    /** `a.e_I(b)` (exclude include) evaluates `a` on the input, and then  
+        - If `a` succeeds, executes `b` on what `a` left behind and returns that result, ignoring `a`.  
+        - If `a` fails, returns that failure instead.  
+        See also `I_e` (include exclude)
+        You can chain the calls e.g.
+
+            a.e_I(b).e_I(c)
+            a.e_I(b.e_I(c))  
+        
+        will parse a, b, c but only return the result of `c`. */
     function e_I<U>(other: B<U>): (p: B<U>)
-      // Excludes the left, includes the right
     {
       B(P.ConcatR(apply, other.apply))
     }
+
+    /** `a.I_e(b)` (include exclude) evaluates `a` on the input, and then  
+        - If `a` succeeds, executes `b` on what `a` left behind.  
+          - If `b` succeeds, returns what `a` parsed along with what `b` left behind.  
+        - If `a` fails, returns that failure.  
+        See also `e_I` (exclude include). You can chain the calls e.g.
+
+            a.I_e(b).I_e(c)
+            a.I_e((b.I_e(c))
+        
+        will parse a, b, c but only return the result of `a`. */
     function I_e<U>(other: B<U>): (p: B<R>)
-      // Includes the left, excludes the right
     {
       B(P.ConcatL(apply, other.apply))
     }
+
+    /** `a.I_I(b)` (include include) evaluates `a` on the input, and then  
+        - If `a` succeeds, executes `b` on what `a` left behind.  
+          - If `b` succeeds, returns a pair of what `a` and `b` resulted with along with what `b` left behind.  
+        - If `a` or `b` fail, returns that failure.  
+        See also `e_I` and `I_e`
+        You can chain the calls e.g.
+
+            a.I_I(b).I_I(c)
+        
+        will parse a, b, c and return the result of `((a, b), c)`. */
     function I_I<U>(other: B<U>): (p: B<(R, U)>)
-      // Includes the left, excludes the right
     {
       B(P.Concat(apply, other.apply))
     }
-    function If<U>(thn: B<U>): (p: B<U>) {
-      B(P.If(apply, thn.apply))
+
+    /** `a.If(cond)` evaluates `cond` on the input, and then if cond returns a success,  
+        evalutes `a` on the original string and returns the result of `a`.  
+        If cond evaluates to a failure, returns the same failure
+        
+        For example, a.If(b.??()) is a way to test the parser b as a lookahead without committing anything.
+         */
+    function If<U>(cond: B<U>): (p: B<R>) {
+      B(P.If(cond.apply, apply))
     }
+
+    /** `a.M(f)` evaluates `a` on the input, and then if it returns a success,  
+        transforms the value using the function `f`. */
     function M<U>(mappingFunc: R -> U): (p: B<U>)
-      // Maps the result
     {
       B(P.Map(apply, mappingFunc))
     }
-    // If the given parser succeeds, moves on to the next.
-    function Commit<V>(other: R -> B<V>): (p: B<V>)
+
+    /** `a.Then(f)` evaluates `a` on the input, and if it is a success,  
+         computes the parser f(result) and executes it on the remaining that `a` did not parse.  
+         The return value is what f(result) returns.  
+         If `a` returns a failure, returns that failure.
+         If `f` is a constant parser b, it is the same as `a.e_I(b)` */
+    function Then<V>(other: R -> B<V>): (p: B<V>)
     {
       B(P.Bind(apply, (result: R) => other(result).apply))
     }
 
-    /** Use a function that can print to debug*/
-    function Debug<D>(name: string, onEnter: (string, P.Input) -> D, onExit: (string, D, P.ParseResult<R>) -> ()): (p: B<R>) {
+    /** `a.ThenWithRemaining(f)` evaluates `a` on the input, and if it is a success,  
+         computes the parser f(result, remainingInput) and executes it on the remaining that `a` did not parse.  
+         The return value is what f(result) returns.  
+         If `a` returns a failure, returns that failure.
+         If `f` is a constant parser b, it is the same as `a.e_I(b)` */
+    function ThenWithRemaining<V>(other: (R, Input) -> B<V>): (p: B<V>)
+    {
+      B(P.BindSucceeds(apply,  (result: R, input: Input) => other(result, input).apply))
+    }
+
+    /** `a.Bind(f)` evaluates `a` on the input.
+         Then it computes the parser f(parse result, original input) and executes it on the remaining that `a` did not parse.  
+         The return value is what f(result) returns.
+         To only bind in case of success, see `a.ThenWithRemaining(_)` or simply `a.Then(_)` */
+    function Bind<V>(other: (ParseResult<R>, Input) -> B<V>): (p: B<V>)
+    {
+      B(P.BindResult(apply, (result: ParseResult<R>, input: Input) => other(result, input).apply))
+    }
+
+    /** `a.Debug(name, onEnter, onExit)` first calls `onEnter(name, input)` when it is executed, obtains the data `d: D`  
+         then it calls `a` on the input (that's the result)
+         then it calls `onExit(name, d, result)`
+         then it return the result.
+         Very useful for debugging, see the README on how to use it. Typically `D` is the input itself. */
+    function Debug<D>(name: string, onEnter: (string, Input) -> D, onExit: (string, D, ParseResult<R>) -> ()): B<R> {
       B(P.Debug(apply, name, onEnter, onExit))
     }
 
-    function Rep<A>(init: A, combine: (A, R) -> A): (p: B<A>)
+    /** `a.RepFold(init, combine) will consider init as an accumulator, and every time `a` succeeds and parses some input, it will
+        combine(init, result) for the new accumulator value.  
+        If `a` fails once while consuming input, it returns the failure. */
+    function RepFold<A>(init: A, combine: (A, R) -> A): (p: B<A>)
     {
       B(P.Rep(apply, combine, init))
     }
 
+    /** `a.RepSep(separator)` returns a sequence of `a` separated by the given separator parser. If the separator parser fails but consumed some input,
+        returns that failure. You might have to suffix your separator with `.??()` if it is a complex separator.
+        `a.RepSep(separator)` is equivalent to
+        `a.?().Then(result => if result.None? then Succeed([]) else
+          separator.e_I(a).Rep([result.a], (acc, newA) => acc + [newA])
+        )`
+        but it's optimized to avoid concatenation of a big sequence with a small one.
+        
+        See `.ZeroOrMore()` if you don't need a separator. */
     function RepSep<K>(separator: B<K>): (p: B<seq<R>>)
     {
       B(P.RepSep(apply, separator.apply))
     }
 
-
+    /** `a.RepMerge(merger)` parses `a` as long as possible and applies the merger on the previous result and the new output.
+      * If `a` cannot be parsed the first time, does not consume any input and returns a recoverable failure.
+      */
     function RepMerge(merger: (R, R) -> R): (p: B<R>)
     {
       B(P.RepMerge(apply, merger))
     }
 
+    /** `a.RepSepMerge(merger)` parses `a` as long as possible and applies the merger on the previous result and the new output,
+      * parsing a potential separator in between.
+      * If `a` cannot be parsed the first time, does not consume any input and returns a recoverable failure.
+      */
     function RepSepMerge<K>(separator: B<K>, merger: (R, R) -> R): (p: B<R>)
     {
       B(P.RepSepMerge(apply, separator.apply, merger))
     }
 
-    function ZeroOrMore(): (p: B<seq<R>>)
+    /** `a.Rep()` keeps parsing `a` as long as the parser consumes some input. It returns a sequence of the parse results.
+      * If returns a failure only if `a` returns a failure that partially parsed the input, or in case of a fatal error. */
+    function Rep(): (p: B<seq<R>>)
     {
       B(P.ZeroOrMore(apply))
     }
 
-    function OneOrMore(): (p: B<seq<R>>)
+    /** `a.Rep1()` keeps parsing `a` as long as the parser consumes some input. It returns a sequence of the parse results.
+      * If returns a failure only if `a` does not parse at the beginning (even if it did not consume any input), or `a` returns a failure that partially parsed the input, or in case of a fatal error. */
+    function Rep1(): (p: B<seq<R>>)
     {
       B(P.OneOrMore(apply))
     }
   }
 
+  /** `O([a, b, ...])` parses `a` on the input, and if `a` succeeds, returns its result.
+      If `a` fails with a fatal error, returns the fatal error.
+      If `a` fails and consumed some input, returns that error.
+      If `a` fails but did not consume any input, continues parsing `b` and so on.
+      If none of the alternatives parse the input, builds a more complex failure message indicating what each sub-parser was expecting.
+  */
   function O<R>(alternatives: seq<B<R>>): B<R>
     // Declares a set of alternatives as a single list
   {
-    if |alternatives| == 0 then Throw("no alternative") else
+    if |alternatives| == 0 then FailWith("no alternative") else
     if |alternatives| == 1 then alternatives[0]
     else
       B(P.Or(alternatives[0].apply, O(alternatives[1..]).apply))
   }
 
-  function End(): B<()>
-  {
-    B(P.EndOfString())
-  }
+  /** `End` succeeds only on an empty string (i.e. the end of the input). */
+  const End: B<()> := B(P.EndOfString())
 
-  function CharTest(test: P.C -> bool, name: string): B<P.C>
+  /** `CharTest(test, name)` tests if the next char of the input satisfies the test, and if so, succeeds with the character.
+      On failure, returns an error message like "expected a {name}" */
+  function CharTest(test: C -> bool, name: string): B<C>
   {
     B(P.CharTest(test, name))
   }
 
+  /** `Rec(a) takes a function that, given a parser, returns a parser.  
+      It provides itself to this function so that makes it possible to create recursive parsers.  
+      For example, to parse nested parentheses like () (()) ... (((((()))))) ..., you can do this:
+      
+          Rec(rec =>
+            O([ 
+              S("(").e_I(rec).I_e(S(")")).M(r => ()),
+              Nothing
+            ]))
+      
+      If on recursion, it detect that no input was consumed, it will raise a fatal error. Therefore, the following parser
+      will return a fatal error on any input
+
+          Rec(rec => rec)
+      
+      and it will explain
+
+          Error: no progress in recursive parser
+  */
   opaque function Rec<R(!new)>(
     underlying: B<R> -> B<R>
   ): B<R>
@@ -156,27 +298,60 @@ abstract module Std.Parsers.Builders {
                     underlying(B(p)).apply))
   }
 
+  /** Datatype used for the values of underlying in `RecMap(underlying, fun)`, see below */
   datatype RecMapDef<!R> = RecMapDef(
     order: nat,
     definition: RecMapSel<R> -> B<R>)
 
+  /** `RecMap(underlying, fun) is a generalization of Rec().
+      underlying is a map from function names to definitions that
+        - Contain a natural order number
+        - Contain a function that accepts a parser and return a parser.
+      The parameter `fun` determines which definition is called first.
+      If a function (e.g. mul) calls a parser (e.g. add) with a greater order number and the same input,
+      it will fail with an error message like
+
+          non-progressing recursive call requires that order of 'add' (3) is lower than the order of 'mul' (2)
+      
+      This guarantees the termination of all parsers.
+      For example, to parse any well-formed expression with parentheses like (), (()(()())), you can do this:
+      
+          RecMap(
+            map[
+              "parens" := RecMapDef(0, rec =>
+                S("(").e_I(rec("list")).I_e(S(")")).M(r => ())
+              ),
+              "list" := RecMapDef(1, rec => O([ 
+                  rec("parens")).I_I(rec("list")).M(r => ())
+                  Epsilon
+                ]))
+              )
+            ],
+            "list")
+      
+      if you try to call into a function that does not exist, it will fail at the time of parsing with a fatal error.
+      If on recursion to a higher order, it detects that no input was consumed, it will raise a fatal error similar to Rec().
+      This construct can be extremely useful for parsing arithmetic expressions.
+  */
   opaque function RecMap<R(!new)>(
     underlying: map<string, RecMapDef<R>>,
     fun: string): (p: B<R>)
   {
     B(P.RecursiveMap(
-        map k <- underlying :: k :=
-                            P.RecursiveDef(
-                              underlying[k].order,
-                              (selector: P.ParserSelector<R>) =>
-                                underlying[k].definition(
-                                  (name: string) =>
-                                    B(selector(name))
-                                ).apply),
+        map k <- underlying ::
+          k :=
+          P.RecursiveDef(
+            underlying[k].order,
+            (selector: P.ParserSelector<R>) =>
+              underlying[k].definition(
+                (name: string) =>
+                  B(selector(name))
+              ).apply),
         fun
       ))
   }
 
+  /** Provides a tool for converting an integer to a string */
   function IntToString(input: int): string {
     P.IntToString(input)
   }
